20250515

src/Automaton.v
@@ -1,9 +1,26 @@
-From mathcomp Require Import fintype seq.
-Require Import MyLib.Basic_Notations_Set.
+From mathcomp Require Import fintype finset seq.
+Require Import MyLib.RelationalCalculus.
 
-Import Rel_Set.
+Module main (def : Relation).
+
+Module Basic_Lemmas := Basic_Lemmas.main(Rel_Set).
+Module Relation_Properties := Relation_Properties.main(Rel_Set).
+Module Functions_Mappings := Functions_Mappings.main Rel_Set.
+Module Dedekind := Dedekind.main Rel_Set.
+Module Conjugate := Conjugate.main Rel_Set.
+Module Domain := Domain.main Rel_Set.
+Module Sum := Sum_Product.main Rel_Set.
+Module Tac := Tactics.main Rel_Set.
+Module Pta := Point_Axiom.main Rel_Set.
+
+Import Rel_Set Basic_Lemmas Relation_Properties Functions_Mappings Dedekind Conjugate Domain Sum Tac Pta.
+Declare Scope automaton_scope.
+Delimit Scope automaton_scope with AUTO.
+Declare Scope language_scope.
+Delimit Scope automaton_scope with LANG.
+
 Structure automaton{state symbol:finType} :=
-    {delta:symbol -> (Rel state state); init:Rel 'I_1 state; final:Rel 'I_1 state}.
+    {delta:symbol -> (Rel state state); init:Rel i state; final:Rel i state}.
 
 Fixpoint dstar{state symbol:finType}(d:symbol -> (Rel state state))(w:seq symbol):(Rel state state):=
 match w with
@@ -11,39 +28,272 @@ match w with
 |s::w' => (d s) ・ (dstar d w')
 end.
 Definition accept{state symbol:finType}(M:@automaton state symbol)(w:seq symbol):Prop :=
-(init M) ・ (dstar(delta M)w) ・ (final M)# = Id 'I_1.
+(init M) ・ (dstar(delta M)w) ・ (final M)# = Id i.
 
-Definition sum_rel{A B C D:eqType}(alpha:Rel A B)(beta:Rel C D):Rel(sum A C)(sum B D):=
-fun x y =>
-    match x, y with
-    | inl a, inl b => alpha a b
-    | inr c, inr d => beta c d
-    | _, _ => False
-    end.
-Definition sum_rel_r{A B C:eqType}(alpha:Rel A B)(beta:Rel A C):Rel A(sum B C):=
-fun x y =>
-    match y with
-    | inl y' => alpha x y'
-    | inr y' => beta x y'
-    end.
+Definition deterministic {state symbol:finType}(M:@automaton state symbol):Prop:=
+(forall s:symbol,function_r(delta M s))/\function_r(init M).
+
 Definition plusM{state1 state2 symbol:finType}(M:@automaton state1 symbol)(M':@automaton state2 symbol):automaton :=
-    {|delta := fun x=>sum_rel((delta M)x)((delta M')x); init:=sum_rel_r(init M)(init M'); final := sum_rel_r(final M)(final M')|}.
+    {|delta := fun x=>(@inl_r state1 state2)#・((delta M)x)・(@inl_r state1 state2)∪((@inr_r state1 state2) #・((delta M')x)・(@inr_r state1 state2)); init:=(init M)・(@inl_r state1 state2)∪((init M')・(@inr_r state1 state2)); final := (final M)・(@inl_r state1 state2)∪((final M')・(@inr_r state1 state2))|}.
+Notation "M '+' M'" := (plusM M M') (at level 50, left associativity, 
+                                      only parsing):automaton_scope.
 
-Lemma lt01:ssrnat.ltn 0 1. Proof. done. Qed.
-Definition o:=Ordinal lt01.
 
-    
-Lemma plusP{state1 state2 symbol:finType}(M:@automaton state1 symbol)(M':@automaton state2 symbol)(w:seq symbol):accept M w\/accept M' w<->accept(plusM M M')w.
+Fixpoint delta_convert'{state:finType}(s:seq state)(R:Rel state state):state->Prop:=
+match s with
+|nil => fun x:state=>False
+|h::s' => fun x:state=>R h x\/delta_convert' s' R x
+end.
+Definition delta_convert{state:finType}(s:{set state})(R:Rel state state):{set state}:=
+[set x|is_true_inv((delta_convert'[seq x <- enum state | x \in s]R)x)].
+
+Theorem NFA_DFA_equiv{symbol:finType}(w:seq symbol):
+(exists (state:finType)(M:@automaton state symbol),accept M w) <-> (exists (state:finType)(M':@automaton state symbol),deterministic M'/\accept M' w).
+split;move=>[state][M];[move=>H|by move=>[_ H];exists state,M].
+exists (finset_set_of__canonical__fintype_Finite state).
+destruct M.
+exists {|delta:= fun (s:symbol)(x y:{set state})=>delta_convert x(delta0 s) = y;
+         init:= fun (x:i)(y:{set state})=>[set x|is_true_inv(init0 tt x)]=y;
+         final:= fun(x:i)(y:{set state})=>y:&:[set x|is_true_inv(final0 tt x)]<>set0|}.
+split.
+rewrite/deterministic.
+split.
+move=>s.
+rewrite/=/function_r/total_r/univalent_r.
+split.
+move=>x y{}H.
+have{}H:y=x;[done|subst].
+by exists (delta_convert x(delta0 s)).
+case=>alpha x.
+case=>y{}H.
+admit. 
+
+
+
+
+Theorem plusP{state1 state2 symbol:finType}(M:@automaton state1 symbol)(M':@automaton state2 symbol)(w:seq symbol):
+accept M w\/accept M' w <-> accept (M+M')%AUTO w.
 Proof.
-    split.
-    case;rewrite/accept=>H.
-    have H1:forall x:state1, (init M)o x -> (init(plusM M M'))o(inl x);[done|].
-    have H2:forall x y:state1, (dstar (delta M) w)x y -> (dstar (delta (plusM M M')) w)(inl x)(inl y).
-    move=>x y{H}.
-    elim w.
-    rewrite/=/identity=>H.
-    by subst.
-    move=>a l H.
-    simpl.
-    rewrite/composite.
+rewrite/accept.
+split.
+case=>H;
+(have:Id i tt tt;[done|]);
+rewrite-{1}H;
+case=>b[]{H};
+case=>a[]H H1 H2;
+apply/inc_antisym_eq;
+(split;[by rewrite unit_identity_is_universal|]=>x y);
+destruct x,y=>_;
+[move:(@inl_id state1 state2)|move:(@inr_id state1 state2)];
+move/inc_antisym_eq=>[_ H3];
+[have H4:Id state1 a a;[done|]|have H4:Id state2 a a;[done|]];
+move:(H3 a a H4)=>{}H4;
+case:H4=>a'[H4 H5];
+[have H6:Id state1 b b;[done|]|have H6:Id state2 b b;[done|]];
+move:(H3 b b H6)=>{}H6;
+case:H6=>b'[H6 H7];
+exists b';
+(split;[exists a';split|]).
+rewrite/=/cup/cupP.
+exists (init M ・ inl_r state1 state2).
+by split;[left|exists a].
+move:a a'{H}H1 H4 H5.
+elim:w.
+simpl=>a a' H.
+have{}H:a=b;[done|].
+subst=>H1{}H2.
+rewrite-inl_inr_cup_id/cup/cupP.
+exists(inl_r state1 state2 # ・ inl_r state1 state2).
+by split;[left|exists b].
+move=>h w H a a'.
+simpl.
+case=>c[H1{}H2 H4 H5].
+have H8:Id state1 c c;[done|].
+move:(H3 c c H8)=>{}H8.
+case:H8=>c'[H8 H9].
+move:(H c c' H2 H8 H9)=>{}H.
+exists c'.
+split.
+rewrite/cup/cupP.
+exists((inl_r state1 state2 # ・ delta M h) ・ inl_r state1 state2).
+by split;[left|exists c;split;[exists a|]].
+done.
+rewrite/=/cup/cupP/inverse.
+exists(final M ・ inl_r state1 state2).
+by split;[left|exists b].
+rewrite/=/cup/cupP.
+exists (init M' ・ inr_r state1 state2).
+by split;[right|exists a].
+move:a a'{H}H1 H4 H5.
+elim:w.
+simpl=>a a' H.
+have{}H:a=b;[done|].
+subst=>H1{}H2.
+rewrite-inl_inr_cup_id/cup/cupP.
+exists(inr_r state1 state2 # ・ inr_r state1 state2).
+by split;[right|exists b].
+move=>h w H a a'.
+simpl.
+case=>c[H1{}H2 H4 H5].
+have H8:Id state2 c c;[done|].
+move:(H3 c c H8)=>{}H8.
+case:H8=>c'[H8 H9].
+move:(H c c' H2 H8 H9)=>{}H.
+exists c'.
+split.
+rewrite/cup/cupP.
+exists((inr_r state1 state2 # ・ delta M' h) ・ inr_r state1 state2).
+by split;[right|exists c;split;[exists a|]].
+done.
+rewrite/=/cup/cupP/inverse.
+exists(final M' ・ inr_r state1 state2).
+by split;[right|exists b].
+
+move=>H;have :Id i tt tt;[done|];rewrite-{1}H.
+case=>b'[].
+case=>a'[].
+case=>alpha[][]{}H;subst=>H H1.
+case=>gamma[][]H2;subst=>H2.
+left.
+case:H=>a[H H3].
+case:H2=>b[H2 H4].
+apply/inc_antisym_eq;
+(split;[by rewrite unit_identity_is_universal|]=>x y);
+destruct x,y=>_.
+exists b.
+split.
+exists a.
+split.
+done.
+move:a' a H3 H1{H}.
+elim:w.
+simpl=>a' a H H1.
+have{}H1:a'=b'.
+done.
+subst.
+rewrite-(@inl_id _ state2).
+by exists b'.
+move=>h w H a' a H1.
+simpl.
+case=>c'[].
+rewrite/cup/cupP.
+case=>alpha[][]H3;subst.
+case=>c[].
+case=>d[]H3.
+have:(inl_r state1 state2 ・ inl_r state1 state2 #) a d.
+by exists a'.
+rewrite inl_id=>H5.
+have{}H5:a=d.
+done.
+subst=>H5 H6 H7.
+move:(H c' c H6 H7)=>{}H.
+by exists c.
+case=>x[].
+case=>y[]H5.
+have:(inl_r state1 state2・inr_r state1 state2 #) a y.
+by exists a'.
+by rewrite inl_inr_empty.
+done.
+
+case:H=>a[]H H3.
+case:H2=>b[]H2 H4.
+exfalso.
+move:a' a{H}H3 H1.
+elim:w.
+move=>a' a H1 H3.
+have{}H5:a'=b'.
+done.
+subst.
+have:(inl_r state1 state2・inr_r state1 state2 #) a b.
+by exists b'.
+by rewrite inl_inr_empty.
+move=>h w H1 a' a H3.
+simpl.
+case=>c'[].
+case=>alpha[][]H5;subst.
+case=>c[]H5 H6 H7.
+by move:(H1 c' c H6 H7).
+case=>x[].
+case=>y[]H5.
+have:(inl_r state1 state2 ・ inr_r state1 state2 #) a y.
+by exists a'.
+by rewrite inl_inr_empty.
+case:H=>a[H H2].
+case=>alpha[][]H3;subst.
+case=>b[]H3 H4.
+exfalso.
+move:w b' b{H3}H4 H1.
+have{}H:(forall (b' : Datatypes_sum__canonical__fintype_Finite state1 state2)
+(b : state1), inl_r state1 state2 b b' ->
+dstar (delta (plusM M M')) nil a' b' -> False).
+move=>b' b{}H H1.
+have H3:a'=b'.
+done.
+subst.
+have:(inr_r state1 state2・inl_r state1 state2 #) a b.
+by exists b'.
+by rewrite inr_inl_empty.
+apply/(last_ind H)=>w t{}H b' b H1.
+have H3:forall (d:symbol->Rel(Datatypes_sum__canonical__fintype_Finite state1 state2)(Datatypes_sum__canonical__fintype_Finite state1 state2))
+(l:seq symbol)(t:symbol), dstar d(rcons l t) = (dstar d l)・(d t).
+move=>d.
+elim.
+move=>t0.
+by rewrite/= comp_id_l comp_id_r.
+move=>h l H3 t0.
+by rewrite/=H3 comp_assoc.
+rewrite{}H3.
+case=>c'[]H3.
+case=>alpha[][]H4;subst.
+case=>c[]H4 H5.
+have:(inl_r state1 state2・inl_r state1 state2 #)b c.
+by exists b'.
+rewrite inl_id=>H6.
+have{}H6:c=b.
+done.
+subst.
+case:H4=>c[]H6.
+by move:(H c' c H6 H3).
+case=>x[_] {}H.
+have:(inl_r state1 state2・inr_r state1 state2 #)b x.
+by exists b'.
+by rewrite inl_inr_empty.
+case=>b[H3 H4].
+right.
+apply/inc_antisym_eq;
+(split;[by rewrite unit_identity_is_universal|]=>x y);
+destruct x,y=>_.
+exists b.
+split;[|done].
+exists a.
+split;[done|].
+move:a' a H2 H1{H H3}.
+elim:w.
+simpl=>a' a H H1.
+have{}H1:b'=a'.
+done.
+subst.
+rewrite-(@inr_id state1).
+by exists a'.
+move=>h w H a' a H1.
+simpl.
+case=>c'[].
+case=>alpha[][]H2;subst.
+case=>c[].
+case=>d[]H2.
+have:(inr_r state1 state2・inl_r state1 state2 #)a d.
+by exists a'.
+by rewrite inr_inl_empty.
+case=>c[].
+case=>d[]H2.
+have{}H2:(inr_r state1 state2・inr_r state1 state2 #)a d.
+by exists a'.
+have{}H2:d=a.
+by rewrite inr_id in H2.
+subst=>{}H1 H2 H3.
+move:(H c' c H2 H3)=>{}H.
+by exists c.
+Qed.
+
+
 
